extract/TestHttp.v
@@ -7,7 +7,7 @@ Parameter command : ocaml_string -> IO int.
 
 Definition run_test : io_unit :=
   IO.unsafe_run
-    (ORandom.self_init tt;; multi_test (@test void http_smi)).
+    (ORandom.self_init tt;; multi_test test_http).
 
 Extract Constant command => "fun s k -> k (Sys.command s)".
 
