ishrink/Common.v
@@ -1,0 +1,35 @@
+From QuickChick Require Export
+     QuickChick.
+From ExtLib Require Export
+     Functor
+     Option.
+From Coq Require Export
+     Basics
+     List.
+Export
+  IfNotations
+  ListNotations.
+
+Definition get {K V} `{Dec_Eq K} (k : K) :
+  list (K * V) -> option V :=
+  fmap snd ∘ find ((fun kv => k = fst kv?)).
+
+Definition delete {K V} `{Dec_Eq K} (k : K) :
+  list (K * V) -> list (K * V) :=
+  filter (fun kv => (k <> fst kv?)).
+
+Definition put {K V} : K -> V -> list (K * V) -> list (K * V) :=
+  compose cons ∘ pair.
+
+Definition update {K V} `{Dec_Eq K} (k : K) (v : V)
+  : list (K * V) -> list (K * V) :=
+  put k v ∘ delete k.
+
+Fixpoint pick {A} (f : A -> bool) (l : list A) : option (A * list A) :=
+  if l is a :: tl
+  then if f a
+       then Some (a, tl)
+       else if pick f tl is Some (x, l')
+            then Some (x, a::l')
+            else None
+  else None.
