ishrink/IShrink.v
@@ -1,0 +1,190 @@
+From IShrink Require Export
+     Common.
+From SimpleIO Require Export
+     SimpleIO.
+From ITree Require Export
+     Exception
+     Nondeterminism
+     ITree.
+From Ceres Require Export
+     Ceres.
+From ExtLib Require Export
+     Extras.
+Export
+  FunNotation
+  FunctorNotation
+  MonadNotation
+  SumNotations.
+Open Scope sum_scope.
+Open Scope string_scope.
+Open Scope list_scope.
+
+Section IShrink.
+
+(** ** Scripting Language *)
+Variable expT               : Type -> Type.
+Variable requestT responseT : (Set -> Type) -> Type.
+Context `{Shrink (requestT expT)}.
+Context `{Serialize (requestT expT)} `{Serialize (responseT id)}.
+
+Definition payloadT exp_ : Type := requestT id + responseT exp_.
+
+Variable connT      : Type.
+Variable Conn__Server : connT.
+Context `{Serialize connT}.
+Context `{Dec_Eq    connT}.
+
+Record packetT {exp_} :=
+  Packet {
+      packet__src : connT;
+      packet__dst : connT;
+      packet__payload : payloadT exp_
+    }.
+Arguments Packet {_}.
+
+Notation pktT := (@packetT id).
+Context `{Serialize pktT}.
+
+Definition labelT := nat.
+
+Definition scriptT := list (labelT * requestT expT).
+Definition traceT  := list (labelT * pktT).
+
+Fixpoint repeat_list {A} (n : nat) (l : list A) : list A :=
+  match n with
+  | O    => []
+  | S n' => l ++ repeat_list n' l
+  end.
+
+Definition shrink_execute' (exec : scriptT -> IO (bool * traceT))
+           (init : scriptT) : IO (option scriptT) :=
+  prerr_endline "<<<<< initial script >>>>>";;
+  prerr_endline (to_string init);;
+  IO.fix_io
+    (fun shrink_rec ss =>
+       match ss with
+       | [] => prerr_endline "<<<<< shrink exhausted >>>>";; ret None
+       | sc :: ss' =>
+         '(b, tr) <- exec sc;;
+         if b : bool
+         then prerr_endline "<<<<< accepting trace >>>>>";;
+              prerr_endline (to_string tr);;
+              shrink_rec ss'
+         else prerr_endline "<<<<< rejecting trace >>>>>";;
+              prerr_endline (to_string tr);;
+              prerr_endline "<<<<< shrink ended >>>>>>>>";;
+              ret (Some sc)
+       end) (repeat_list 20 $ shrink init).
+
+Definition shrink_execute (first_exec : IO (bool * (scriptT * traceT)))
+           (then_exec : scriptT -> IO (bool * traceT)) : IO bool :=
+  '(b, (sc, _)) <- first_exec;;
+  if b : bool
+  then ret true
+  else IO.while_loop (shrink_execute' then_exec) sc;;
+       ret false.
+
+(** ** Testing Language *)
+
+Variable gen_state : Type.
+
+Variant clientE : Type -> Type :=
+  Client__Recv : clientE (option pktT)
+| Client__Send : gen_state -> clientE (option pktT).
+
+Variable otherE : Type -> Type.
+Variable other_handler : otherE ~> IO.
+Arguments other_handler {_}.
+
+Definition failureE := (exceptE string).
+Notation tE := (failureE +' clientE +' otherE).
+
+Variable instantiate_request : traceT -> requestT expT -> requestT id.
+Variable gen_request   : gen_state -> traceT -> IO (requestT expT).
+Variable conn_state    : Type.
+Variable init_state    : conn_state.
+Variable recv_response : Monads.stateT conn_state IO (option pktT).
+Variable send_request  :
+  requestT id -> Monads.stateT conn_state IO (option connT).
+
+Fixpoint execute' {R} (fuel : nat) (s : conn_state)
+         (oscript : option scriptT) (acc : scriptT * traceT) (m : itree tE R)
+  : IO (bool * conn_state * (scriptT * traceT)) :=
+  let (script0, trace0) := acc in
+  match fuel with
+  | O => ret (true, s, acc)
+  | S fuel =>
+    match observe m with
+    | RetF _ => ret (true, s, acc)
+    | TauF m' => execute' fuel s oscript acc m'
+    | VisF e k =>
+      match e with
+      | (Throw err|) => ret (false, s, acc)
+      | (|ce|) =>
+        match ce in clientE Y return (Y -> _) -> _ with
+        | Client__Recv =>
+          fun k => '(s', op) <- recv_response s;;
+                let acc' :=
+                    match op with
+                    | Some p =>
+                      let dst : connT := packet__dst p in
+                      let lreqs :=
+                          filter (fun lpkt => packet__src (snd lpkt) = dst?)
+                                 trace0 in
+                      let prevs :=
+                          length (filter (fun lpkt => packet__dst (snd lpkt) = dst?)
+                                         trace0) in
+                      let label := nth prevs (map fst lreqs) O in
+                      (script0, trace0 ++ [(label, p)])
+                    | None => acc
+                    end in
+                execute' fuel s' oscript acc' (k op)
+        | Client__Send gs =>
+          fun k => '(ostep, osc') <-
+                match oscript with
+                | Some [] => ret (None, Some [])
+                | Some (sc :: script') =>
+                  ret (Some sc, Some script')
+                | None =>
+                  let freshVar : nat :=
+                      S $ fold_left Nat.max (map fst script0) O in
+                  step <- pair freshVar <$> gen_request gs trace0;;
+                         ret (Some step, None)
+                end;;
+                match ostep with
+                | Some ((n, rx) as step) =>
+                  let req : requestT id := instantiate_request trace0 rx in
+                  '(s', oc) <- send_request req s;;
+                  if oc is Some c
+                  then let pkt : pktT := Packet c Conn__Server (inl req) in
+                       execute' fuel s' osc'
+                                (script0 ++ [step], trace0 ++ [(n, pkt)])
+                                (k (Some pkt))
+                  else execute' fuel s' osc' acc (k None)
+                | None => execute' fuel s osc' acc (k None)
+                end
+        end k
+      | (||oe) => other_handler oe >>= execute' fuel s oscript acc ∘ k
+      end
+    end
+  end.
+
+Variable cleanup : conn_state -> IO unit.
+
+Definition execute {R} (m : itree tE R) (oscript : option scriptT)
+  : IO (bool * (scriptT * traceT)) :=
+  '(b, s, t') <- execute' 5000 init_state oscript ([], []) m;;
+  cleanup s;;
+  ret (b, t').
+
+Definition test {R} (m : itree tE R) : IO bool :=
+  shrink_execute (execute m None)
+                 (fmap (fun '(b, (_, t)) => (b, t)) ∘ execute m ∘ Some).
+
+End IShrink.
+
+Arguments packetT : clear implicits.
+Arguments Packet        {_ _ _ _}.
+Arguments packet__src     {_ _ _ _}.
+Arguments packet__dst     {_ _ _ _}.
+Arguments packet__payload {_ _ _ _}.
