theories/Instances.v
@@ -1,78 +1,16 @@
+From QuickChick Require Import
+     Decidability.
 From HTTP Require Import
-     Common
      Message.
 
-Program Instance Decidable_eq_method (x y : request_method) : Decidable (x = y) := {
-  Decidable_witness :=
-    match x, y with
-    | Method__GET    , Method__GET
-    | Method__HEAD   , Method__HEAD
-    | Method__POST   , Method__POST
-    | Method__PUT    , Method__PUT
-    | Method__DELETE , Method__DELETE
-    | Method__CONNECT, Method__CONNECT
-    | Method__OPTIONS, Method__OPTIONS
-    | Method__TRACE  , Method__TRACE => true
-    | Method sx    , Method sy => sx = sy?
-    | _, _ => false
-    end }.
-Solve Obligations with split; intuition; try discriminate.
-Next Obligation.
-  intuition.
-  - destruct x, y; try discriminate; intuition.
-    f_equal.
-    apply eqb_eq.
-    assumption.
-  - subst.
-    destruct y; intuition.
-    apply eqb_eq.
-    reflexivity.
-Qed.
+Instance Dec_Eq__method : Dec_Eq request_method.
+Proof. dec_eq. Defined.
 
-Program Instance Decidable_eq_scheme (x y : http_scheme) : Decidable (x = y) :=
-  { Decidable_witness :=
-      match x, y with
-      | Scheme__HTTP , Scheme__HTTP
-      | Scheme__HTTPS, Scheme__HTTPS => true
-      | Scheme s1  , Scheme s2 => s1 = s2?
-      | _, _ => false
-      end }.
-Solve Obligations with split; intuition; discriminate.
-Next Obligation.
-  destruct x, y; intuition; try discriminate; f_equal; apply eqb_eq; intuition.
-  inversion H; reflexivity.
-Qed.
+Instance Dec_Eq__scheme : Dec_Eq http_scheme.
+Proof. dec_eq. Defined.
 
-Program Instance Decidable_eq_authority (x y : authority) : Decidable (x = y) :=
-  { Decidable_witness :=
-      let 'Authority u1 h1 p1 := x in
-      let 'Authority u2 h2 p2 := y in
-      (u1 = u2?) &&& (h1 =? h2) &&& (p1 = p2?) }.
-Next Obligation.
-  intuition.
-  - destruct x, y.
-    do 2 (apply andb_true_iff in H; destruct H).
-    f_equal; apply Decidable_spec; intuition.
-  - subst.
-    destruct y.
-    destruct authority__userinfo, authority__port;
-      repeat (apply andb_true_iff; intuition);
-        try apply eqb_eq; try apply N.eqb_eq; reflexivity.
-Qed.
+Instance Dec_Eq__authority : Dec_Eq authority.
+Proof. dec_eq. Defined.
 
-Program Instance Decidable_eq_uri (x y : absolute_uri) : Decidable (x = y) :=
-  { Decidable_witness :=
-      let 'URI s1 a1 p1 oq1 := x in
-      let 'URI s2 a2 p2 oq2 := y in
-      (s1 = s2)? &&& (a1 = a2?) &&& (p1 =? p2) &&& (oq1 = oq2?) }.
-Next Obligation.
-  intuition.
-  - destruct x, y.
-    do 3 (apply andb_true_iff in H; destruct H).
-    f_equal; apply Decidable_spec; intuition.
-  - subst.
-    destruct y.
-    destruct uri__scheme, uri__authority, uri__query, authority__userinfo, authority__port;
-      repeat (apply andb_true_iff; intuition);
-      try apply eqb_eq; try apply N.eqb_eq; reflexivity.
-Qed.
+Instance Dec_Eq__uri : Dec_Eq absolute_uri.
+Proof. dec_eq. Defined.
