theories/NetUnix.v
@@ -3,8 +3,7 @@ From Coq Require Export
      String.
 From ExtLib Require Export
      Functor
-     Monad
-     StateMonad.
+     Monad.
 From SimpleIO Require Export
      IO_Bytes
      IO_Float
@@ -28,9 +27,6 @@ Import
 
 Coercion int_of_n : N >-> int.
 
-Definition getport : IO N :=
-  N.add 8000 ∘ n_of_int <$> ORandom.int 5000.
-
 Definition try {a b} (f : IO a) (g : IO b) : IO (option a) :=
   catch_error
     (Some <$> f) $
@@ -41,63 +37,34 @@ Definition try {a b} (f : IO a) (g : IO b) : IO (option a) :=
       (*                            error_message e);; *)
       ret None.
 
-Definition create_sock' (port : N) : IO (option file_descr) :=
-  let iaddr : inet_addr := inet_addr_any in
-  ofd <- try (socket PF_INET SOCK_STREAM int_zero) (ret tt);;
-  match ofd with
-  | Some fd =>
-    let f :=
-        bind fd (ADDR_INET iaddr $ int_of_n port);;
-        listen fd 128;;
-        ret fd in
-    try f $
-        (* prerr_endline ("Binding and listening to port " *)
-        (*                  ++ to_string port);; *)
-    close fd
-  | None => ret None
-  end.
-
-Definition create_sock : IO (N * file_descr) :=
-  getport >>=
-          IO.fix_io
-          (fun next p =>
-             ofd <- create_sock' p;;
-             match ofd with
-             | Some fd => ret (p, fd)
-             | None    => getport >>= next
-             end).
-
-Definition accept_conn (sfd : file_descr) : IO file_descr :=
-  fst <$> accept sfd.
-
 Definition conn_state := list (clientT * (file_descr * string)).
 
 Definition conn_of_fd (fd : file_descr)
   : conn_state -> option (clientT * (file_descr * string)) :=
   find (file_descr_eqb fd ∘ fst ∘ snd).
 
-Definition create_conn (c : clientT) : stateT conn_state IO (option file_descr) :=
-  mkStateT
-    (fun s =>
-       let iaddr : inet_addr := inet_addr_loopback in
-       ofd <- try (fd <- socket PF_INET SOCK_STREAM int_zero;;
-                  connect fd (ADDR_INET iaddr server_port);;
-                  ret fd) (ret tt);;
-       ret (ofd, match ofd with
-                 | Some fd => (c, (fd, ""))::s
-                 | None    => s
-                 end)).
+Definition create_conn (s : conn_state)
+  : IO (conn_state * option (file_descr * clientT)) :=
+  let iaddr : inet_addr := inet_addr_loopback in
+  ofd <- try (fd <- socket PF_INET SOCK_STREAM int_zero;;
+             connect fd (ADDR_INET iaddr server_port);;
+             ret fd) (ret tt);;
+  match ofd with
+  | Some fd =>
+    let c := length s in
+    ret ((c, (fd, ""))::s, Some (fd, c))
+  | None => ret (s, None)
+  end.
 
 Notation BUFFER_SIZE := 1024.
 Definition SELECT_TIMEOUT := OFloat.Unsafe.of_string "0".
 
-Definition recv_bytes' : stateT conn_state IO bool :=
-  mkStateT
+Definition recv_bytes' : Monads.stateT conn_state IO bool :=
     (fun s =>
        '(fds, _, _) <- select (map (fst ∘ snd) s) [] [] SELECT_TIMEOUT;;
        fold_left
          (fun _bs0 fd =>
-            '(b, s0) <- _bs0;;
+            '(s0, b) <- _bs0;;
             match conn_of_fd fd s0 with
             | Some (c, (fd, str0)) =>
               buf <- OBytes.create BUFFER_SIZE;;
@@ -108,66 +75,23 @@ Definition recv_bytes' : stateT conn_state IO bool :=
                    then _bs0
                    else str <- from_ostring <$> OBytes.to_string buf;;
                         let str1 : string := substring 0 (nat_of_int len) str in
-                        ret (true, update c (fd, str0 ++ str1) s0)
+                        ret (update c (fd, str0 ++ str1) s0, true)
             | None => _bs0
-            end)%int fds (ret (false, s))).
+            end)%int fds (ret (s, false))).
 
-Definition recv_bytes : stateT conn_state IO unit :=
-  mkStateT
+Definition recv_bytes : Monads.stateT conn_state IO unit :=
     (IO.fix_io
        (fun recv_rec s =>
-          '(b, s') <- runStateT recv_bytes' s;;
-          if b : bool then recv_rec s' else ret (tt, s'))).
+          '(s', b) <- recv_bytes' s;;
+          if b : bool then recv_rec s' else ret (s', tt))).
 
 Instance Serialize__conn : Serialize (file_descr * string) :=
   to_sexp ∘ snd.
 
-Definition origin_state : Type :=
-  file_descr * N *
-  list (clientT *
-        (file_descr * string * option (http_request id))) *
-  server_state id.
-
-Definition origin_host (port : N) : authority :=
-  Authority None "host.docker.internal" (Some port).
-
-Definition proxy_of_fd (fd : file_descr)
-  : list (clientT * (file_descr * string * option (http_request id))) ->
-    option (clientT * (file_descr * string * option (http_request id))) :=
-  find (file_descr_eqb fd ∘ fst ∘ fst ∘ snd).
-
-Definition recv_bytes_origin : stateT origin_state IO unit :=
-  mkStateT
-    $ fun s =>
-        let '(sfd, port, conns, ss) := s in
-        '(fds, _, _) <- select (map (fst ∘ fst ∘ snd) conns) [] [] SELECT_TIMEOUT;;
-        conns' <-
-        fold_left
-          (fun _s0 fd =>
-             s0 <- _s0;;
-             match proxy_of_fd fd s0 with
-             | Some (c, (fd, str0, or)) =>
-               buf <- OBytes.create BUFFER_SIZE;;
-               len <- recv fd buf int_zero BUFFER_SIZE [];;
-               if len <? int_zero
-               then close fd;; ret s0
-               else if len =? int_zero
-                    then _s0
-                    else str <- from_ostring <$> OBytes.to_string buf;;
-                         let str1 : string := substring 0 (nat_of_int len) str in
-                         ret $ update c (fd, str0 ++ str1, or) s0
-             | None => ret s0
-             end)%int fds
-          ('(fds, _, _) <- select [sfd] [] [] SELECT_TIMEOUT;;
-           match fds with
-           | [] => ret conns
-           | sfd :: _ => fd <- accept_conn sfd;;
-                       ret (put (length conns) (fd, "", None) conns)
-           end);;
-        ret (tt, (sfd, port, conns', ss)).
-
-Definition send_request (c : clientT) (req : http_request id) : stateT conn_state IO bool :=
-  let send_bytes fd s :=
+Definition send_request (req : http_request id)
+  : Monads.stateT conn_state IO (option connT) :=
+  let send_bytes fdc s : IO (conn_state * option connT) :=
+        let (fd, c) := fdc : file_descr * clientT in
         let str : string := request_to_string req in
         buf <- OBytes.of_string str;;
         let len : int := OBytes.length buf in
@@ -177,49 +101,18 @@ Definition send_request (c : clientT) (req : http_request id) : stateT conn_stat
              if sent <? int_zero
              then close fd;;
                   (* prerr_endline "Send byte failed";; *)
-                  ret false
+                  ret None
              else
                if o + sent =? len
                then
-                 prerr_endline ("================SENT================"
-                                     ++ to_string c ++ CRLF ++ str);;
-                 ret true
+                 (* prerr_endline ("================SENT================" *)
+                 (*                     ++ to_string c ++ CRLF ++ str);; *)
+                 ret (Some (Conn__User c))
                else send_rec (o + sent))%int int_zero;;
-        ret (b, s)
+        ret (s, None)
   in
-  mkStateT
     (fun s =>
-         match get c s with
-         | Some (fd, _) => send_bytes fd s
-         | None => '(ofd, s') <- runStateT (create_conn c) s;;
-                  match ofd with
-                  | Some fd => send_bytes fd s'
-                  | None    => ret (false, s')
-                  end
-         end).
-
-Definition send_response (c : clientT) (res : http_response id) : stateT origin_state IO bool :=
-  mkStateT
-    (fun s =>
-       let '(sfd, port, conns, ss) := s in
-       match get c conns with
-       | Some (fd, _, _) =>
-         let str : string := response_to_string res in
-         buf <- OBytes.of_string str;;
-         let len : int := OBytes.length buf in
-         b <- IO.fix_io
-               (fun send_rec o =>
-                  sent <- send fd buf o (len - o)%int [];;
-                  if sent <? int_zero
-                  then ret false
-                  else
-                    if o + sent =? len
-                    then
-                      prerr_endline ("=============PROXY SENT============="
-                                       ++ to_string c
-                                       ++ CRLF ++ str);;
-                      ret true
-                    else send_rec (o + sent))%int int_zero;;
-         ret (b, s)
-       | None => ret (false, s)
-       end).
+       '(s', ofdc) <- create_conn s;;
+       if ofdc is Some fdc
+       then send_bytes fdc s'
+       else ret (s', None)).
